src/Compilers/Tuple.v
@@ -44,19 +44,23 @@ Section language.
       Lemma flat_interp_tuple_untuple {T n v}
         : @flat_interp_tuple T n (flat_interp_untuple v) = v.
       Proof using Type. destruct n; [ reflexivity | apply flat_interp_tuple'_untuple' ]. Qed.
-
-      Definition tuple_map {A B n} (f : interp_flat_type A -> interp_flat_type B) (v : interp_flat_type (tuple A n))
-        : interp_flat_type (tuple B n)
-        := let fv := Tuple.map f (flat_interp_tuple v) in
-           match n return interp_flat_type (tuple A n) -> Tuple.tuple (interp_flat_type B) n -> interp_flat_type (tuple B n) with
-           | 0 => fun v x => x
-           | S _ => fun v fv => flat_interp_untuple' fv
-           end v fv.
     End flat_type.
   End interp.
+
+  Section interp2.
+    Section flat_type.
+      Context {interp_base_type1 interp_base_type2 : base_type_code -> Type}.
+      Local Notation interp_flat_type1 := (interp_flat_type interp_base_type1).
+      Local Notation interp_flat_type2 := (interp_flat_type interp_base_type2).
+
+      Definition tuple_map {A B n} (f : interp_flat_type1 A -> interp_flat_type2 B) (v : interp_flat_type1 (tuple A n))
+        : interp_flat_type2 (tuple B n)
+        := flat_interp_untuple (Tuple.map f (flat_interp_tuple v)).
+    End flat_type.
+  End interp2.
 End language.
 Global Arguments flat_interp_tuple' {_ _ _ _} _.
 Global Arguments flat_interp_tuple {_ _ _ _} _.
 Global Arguments flat_interp_untuple' {_ _ _ _} _.
 Global Arguments flat_interp_untuple {_ _ _ _} _.
-Global Arguments tuple_map {_ _ _ _ n} _ _.
+Global Arguments tuple_map {_ _ _ _ _ n} _ _.
